new/proof/strings.v
@@ -2,6 +2,7 @@ From New.proof Require Import proof_prelude.
 From New.proof Require Export std.
 From New.generatedproof Require Export strings.
 From Perennial Require Import base.
+From Coq Require Import PropExtensionality.
 
 Section wps.
 Context `{hG: heapGS Σ, !ffi_semantics _ _}.
@@ -19,6 +20,120 @@ Lemma wp_asciiSpace_init :
 Proof.
 Admitted.
 
+Fixpoint go_string_ltb (x y : go_string) : bool :=
+  match x, y with
+  | [], [] => false
+  | [], _ => true
+  | _, [] => false
+  | (a :: x), (b :: y) => if (word.ltu a b) then
+                         true
+                       else if (word.eqb a b) then
+                              go_string_ltb x y
+                            else false
+  end.
+
+Example go_string_ltb_examples :
+  go_string_ltb "" "" = false ∧
+  go_string_ltb "" "a" = true ∧
+  go_string_ltb "a" "" = false ∧
+  go_string_ltb "ab" "a" = false ∧
+  go_string_ltb "ab" "b" = true
+  := ltac:(auto).
+
+Fixpoint go_string_lt (x y : go_string) : Prop :=
+  match x, y with
+  | [], [] => False
+  | [], _ => True
+  | _, [] => False
+  | (a :: x), (b :: y) => if decide (uint.Z a < uint.Z b) then
+                         True
+                       else if decide (uint.Z a = uint.Z b) then
+                              go_string_lt x y
+                            else false
+  end.
+
+Definition go_string_le (x y : go_string) : Prop :=
+  x = y ∨ go_string_lt x y.
+
+Definition go_string_leb (x y : go_string) : bool :=
+ bool_decide(x = y) || go_string_ltb x y.
+
+Lemma w8_trichotomy (a b : w8) :
+  word.ltu a b = true \/ word.eqb a b = true \/ word.ltu b a = true.
+Proof.
+  destruct (decide (uint.Z a < uint.Z b)%Z) as [Hab|Hnab].
+  - left.
+    rewrite word.unsigned_ltu.
+    apply Z.ltb_lt.
+    exact Hab.
+  - destruct (decide (uint.Z a = uint.Z b)%Z) as [Heq|Hneq].
+    + right. left.
+      apply word.eqb_eq. 
+      word.
+    + right. right.
+      assert ((uint.Z b < uint.Z a)%Z) by lia.
+      rewrite word.unsigned_ltu.
+      apply Z.ltb_lt.
+      assumption.
+Qed.
+
+Lemma w8_ltu_irrefl (a : w8) :
+  word.ltu a a = false.
+Proof.
+  rewrite word.unsigned_ltu. 
+  apply Z.ltb_irrefl.
+Qed.
+
+Lemma w8_eqb_refl (a : w8) :
+  word.eqb a a = true.
+Proof.
+  apply word.eqb_eq. done.
+Qed.
+
+Lemma go_string_ltb_total x y :
+  x = y \/ go_string_ltb x y = true \/ go_string_ltb y x = true.
+Proof.
+  revert y.
+  induction x as [|a x IH]; intros [|b y].
+  - left; reflexivity.
+  - right; left; reflexivity.
+  - right; right; reflexivity.
+  - destruct (w8_trichotomy a b) as [Hlt | [Heq | Hgt]].
+    + right; left; simpl; rewrite Hlt; reflexivity.
+    + destruct (word.eqb_spec a b) as [Hab | Hab].
+      * subst.
+        destruct (IH y) as [Hxy | [Hxy | Hxy]].
+        -- left; congruence.
+        -- right; left; simpl; rewrite w8_ltu_irrefl. rewrite w8_eqb_refl; assumption.
+        -- right; right; simpl; rewrite w8_ltu_irrefl. rewrite w8_eqb_refl; assumption.
+      * exfalso. apply Hab. done.
+    + right; right; simpl; rewrite Hgt; reflexivity.
+Qed.
+
+Lemma go_string_leb_total x y :
+  go_string_leb x y = true \/ go_string_leb y x = true.
+Proof.
+  destruct (go_string_ltb_total x y) as [-> | [Hxy | Hyx]].
+  - left.
+    unfold go_string_leb.
+    assert (y = y) by done. 
+    assert (bool_decide (y = y)) by set_solver.  
+    replace (bool_decide (y = y)) with true.
+    { done. } rewrite bool_decide_true. { done. } done.
+  - left.
+    unfold go_string_leb.
+    replace (go_string_ltb x y ) with true. 
+    replace (true = true) with True;first lia. 
+    apply Coq.Logic.PropExtensionality.propositional_extensionality; naive_solver.
+  
+  - right.
+    unfold go_string_leb.
+
+    rewrite Hyx. 
+    replace (true = true) with True;first lia. 
+    apply Coq.Logic.PropExtensionality.propositional_extensionality; naive_solver.
+Qed.
+
 Lemma wp_initialize' get_is_pkg_init :
   get_is_pkg_init_prop strings get_is_pkg_init →
   {{{ own_initializing get_is_pkg_init }}}
@@ -31,6 +146,118 @@ Proof.
   iIntros "Hown". wp_auto.
   wp_apply wp_asciiSpace_init.
   iEval (rewrite is_pkg_init_unfold /=). iFrame "∗#". done.
+Qed.
+
+Definition is_space_byte (b : w8) : bool :=
+  (word.eqb b (W8 32)) ||    (* space    *)
+  (word.eqb b (W8 9))  ||    (* \t       *)
+  (word.eqb b (W8 10)) ||    (* \n       *)
+  (word.eqb b (W8 13)).      (* \r       *)
+
+Fixpoint drop_while {A} (f : A -> bool) (xs : list A) : list A :=
+  match xs with
+  | [] => []
+  | x :: xs' => if f x then drop_while f xs' else x :: xs'
+  end.
+
+Fixpoint take_while {A} (f : A -> bool) (xs : list A) : list A :=
+  match xs with
+  | [] => []
+  | x :: xs' => if f x then x :: take_while f xs' else []
+  end.
+
+Fixpoint split_fields_go (fuel : nat) (s : go_string) : list go_string :=
+  match fuel with
+  | O => []
+  | S fuel' =>
+      let s' := drop_while is_space_byte s in
+      match s' with
+      | [] => []
+      | _ =>
+          let w := take_while (fun b => negb (is_space_byte b)) s' in
+          let rest := drop_while (fun b => negb (is_space_byte b)) s' in
+          w :: split_fields_go fuel' rest
+      end
+  end.
+
+Definition fields_spec (s : go_string) (ss : list go_string) : Prop :=
+  ss = split_fields_go (length s) s ∧ (length ss) < 2 ^ 64 .
+
+Axiom wp_strings_Fields :
+  ∀ `{!strings.Assumptions} (s : go_string),
+  {{{ is_pkg_init strings }}}
+    @! strings.Fields #s
+  {{{ sl (ss : list go_string),
+      RET #sl;
+      sl ↦* ss ∗ ⌜ fields_spec s ss ⌝ ∗  own_slice_cap w8 sl (DfracOwn 1) }}}.
+
+Example split_fields_go_hello :
+  split_fields_go (length "hello"%go) "hello"%go = ["hello"%go].
+Proof. vm_compute. reflexivity. Qed.
+
+Example split_fields_go_leading_spaces :
+  split_fields_go (length "   hello world"%go) "   hello world"%go =
+    ["hello"%go; "world"%go].
+Proof. vm_compute. reflexivity. Qed.
+
+Example split_fields_go_two_words :
+  split_fields_go (length "hello world"%go) "hello world"%go =
+    ["hello"%go; "world"%go].
+Proof. vm_compute. reflexivity. Qed.
+
+Example split_fields_go_empty :
+  split_fields_go (length ""%go) ""%go = [].
+Proof. vm_compute. reflexivity. Qed.
+
+Definition bs_tab : w8 := W8 9.
+Definition bs_nl  : w8 := W8 10.
+Definition bs_cr  : w8 := W8 13.
+Definition bs_sp  : w8 := W8 32.
+
+Definition hello_world_ws : go_string :=
+  [bs_sp; bs_tab] ++ "hello"%go ++ [bs_nl] ++ "world"%go ++ [bs_cr; bs_sp].
+
+Example split_fields_go_mixed_ws :
+  split_fields_go (length hello_world_ws) hello_world_ws =
+    ["hello"%go; "world"%go].
+Proof. vm_compute. reflexivity. Qed.
+
+Example split_fields_go_interp_string_literal :
+  split_fields_go (length "  hello\tthere\ngeneral\rkenobi "%go)
+                  "  hello\tthere\ngeneral\rkenobi "%go
+  = ["hello"%go; "there"%go; "general"%go; "kenobi"%go].
+Proof. vm_compute. reflexivity. Qed.
+
+Example wp_Fields_mixed_ws :
+  {{{ is_pkg_init strings }}}
+    @! strings.Fields #("  hello\tthere\ngeneral\rkenobi "%go)
+  {{{ sl,
+      RET #sl;
+      sl ↦* ["hello"%go; "there"%go; "general"%go; "kenobi"%go] ∗ own_slice_cap w8 sl (DfracOwn 1) }}}.
+Proof.
+  iIntros (Φ) "#Hinit HΦ".
+  wp_apply (wp_strings_Fields).
+  iIntros (sl ss) "(Hsl & %Hspec & Hcap)".
+  destruct Hspec as [Hss _].
+  subst ss.
+  iApply "HΦ". iFrame.
+Qed.
+
+Example wp_Fields_two_words:
+  {{{ is_pkg_init strings }}}
+    @! strings.Fields #"hello world"%go
+  {{{ sl,
+      RET #sl;
+      sl ↦* ["hello"%go; "world"%go] ∗
+      own_slice_cap w8 sl (DfracOwn 1) 
+  }}}.
+Proof.
+  iIntros (Φ) "#Hinit HΦ".
+  wp_apply (wp_strings_Fields "hello world"%go).
+  iIntros (sl ss) "(Hsl & %Hspec & Hcap)".
+  destruct Hspec as [Hss _].
+  subst ss.
+  iApply "HΦ". iFrame.
 Qed.
 
 End wps.
